Substitution functions for every variable at once

theories/Closed.v
@@ -1,48 +1,23 @@
 From Coq Require Export
   Lists.List.
 Export ListNotations.
-From Adam Require Import
+From Lang Require Import
   Invert
   OptionBind
   Snoc
-  Terms
-  Types.
+  Terms.
 
-(*
-(* Free variables under a given context (without types).
- * Returns all free variables in reverse order. *)
-Fixpoint fv_under ctx acc t :=
-  match t with
-  | TmVoid
-  | TmStar _
-  | TmAtom _ _ =>
-      (ctx, acc)
-  | TmVarS s =>
-      match ctx with
-      | hd :: tl => if eqb s hd then (tl, acc) else (ctx, s :: acc)
-      | [] => (ctx, s :: acc)
-      end
-  | TmPack _ None a b
-  | TmForA None a b
-  | TmAppl a b => 
-      let (ctmp, atmp) := fv_under ctx acc a in
-      fv_under ctmp atmp b
-  | TmPack _ (Some arg) ty curry
-  | TmForA (Some arg) ty curry => 
-      let (ctmp, atmp) := fv_under ctx acc ty in
-      fv_under (arg :: ctmp) atmp curry
+Fixpoint destructive_search needle haystack :=
+  match haystack with
+  | [] => None
+  | hd :: tl => if eqb needle hd then Some tl else destructive_search needle tl
   end.
-Definition fv : term -> list string := fun t => let (_, f) := fv_under [] [] t in f.
-Arguments fv t/.
-Definition closed : term -> bool := fun t => match fv t with [] => true | _ :: _ => false end.
-Arguments closed t/.
-*)
 
 Fixpoint fv_slow t :=
   match t with
   | TmVoid
-  | TmStar _
-  | TmAtom _ _ =>
+  | TmStar
+  | TmAtom _ =>
       []
   | TmVarS s =>
       [s]
@@ -58,11 +33,29 @@ Fixpoint fv_slow t :=
       | hd :: tl => if eqb arg hd then tl else hd :: tl
       end
   end.
+
+(* Crucial distinction from an easier-to-implement algorithm! *)
+Example fv_slow_permits_shadowing : forall x,
+  (* Equivalent to `\x. \x. x x`, where the `x`s are distinct and pushed/popped in order. *)
+  fv_slow (TmForA (Some x) TmVoid (TmForA (Some x) TmVoid (TmAppl (TmVarS x) (TmVarS x)))) = [].
+Proof. intros. simpl. repeat rewrite eqb_refl. reflexivity. Qed.
+
+(* Crucial distinction from an easier-to-implement algorithm! *)
+Example fv_slow_permits_interrupted_shadowing : forall x y, y <> x ->
+  (* Equivalent to `\x. \y. \x. x x`, where the `x`s are distinct and pushed/popped in order. *)
+  fv_slow (TmForA (Some x) TmVoid (TmForA (Some y) TmVoid (TmForA (Some x) TmVoid (TmAppl (TmVarS x) (TmVarS x))))) = [].
+Proof. intros. apply eqb_neq in H. simpl. rewrite eqb_refl. rewrite H. rewrite eqb_refl. reflexivity. Qed.
+
+Example fv_slow_respects_scope : forall x,
+  (* Equivalent to `(\x:0. 0) x`, in which the outer `x` is still free *)
+  fv_slow (TmAppl (TmForA (Some x) TmVoid TmVoid) (TmVarS x)) = [x].
+Proof. intros. simpl. reflexivity. Qed.
+
 Fixpoint fv_fast acc t :=
   match t with
   | TmVoid
-  | TmStar _
-  | TmAtom _ _ =>
+  | TmStar
+  | TmAtom _ =>
       acc
   | TmVarS s =>
       s :: acc
@@ -72,32 +65,57 @@ Fixpoint fv_fast acc t :=
       fv_fast (fv_fast acc b) a
   | TmPack _ (Some arg) ty curry
   | TmForA (Some arg) ty curry =>
-      match fv_fast (fv_fast acc curry) ty with
+      let tmp := match fv_fast acc curry with
       | [] => []
       | hd :: tl => if eqb arg hd then tl else hd :: tl
-      end
+      end in
+      fv_fast tmp ty
   end.
 
-Lemma fv_fast_acc_app : forall acc t,
-  fv_fast acc t = fv_fast [] t ++ acc.
-Proof.
-  intros. generalize dependent acc. induction t; intros; simpl in *;
-  simpl in *; try reflexivity.
-  - destruct arg; rewrite IHt1; rewrite (IHt1 (fv_fast [] t2)); rewrite IHt2; [| rewrite app_assoc; reflexivity].
-    (* FUCK *) Abort.
+(* Crucial distinction from an easier-to-implement algorithm! *)
+Example fv_fast_permits_shadowing : forall x,
+  (* Equivalent to `\x. \x. x x`, where the `x`s are distinct and pushed/popped in order. *)
+  fv_fast [] (TmForA (Some x) TmVoid (TmForA (Some x) TmVoid (TmAppl (TmVarS x) (TmVarS x)))) = [].
+Proof. intros. simpl. repeat rewrite eqb_refl. reflexivity. Qed.
+
+(* Crucial distinction from an easier-to-implement algorithm! *)
+Example fv_fast_permits_interrupted_shadowing : forall x y, y <> x ->
+  (* Equivalent to `\x. \y. \x. x x`, where the `x`s are distinct and pushed/popped in order. *)
+  fv_fast [] (TmForA (Some x) TmVoid (TmForA (Some y) TmVoid (TmForA (Some x) TmVoid (TmAppl (TmVarS x) (TmVarS x))))) = [].
+Proof. intros. apply eqb_neq in H. simpl. rewrite eqb_refl. rewrite H. rewrite eqb_refl. reflexivity. Qed.
+
+Example fv_fast_respects_scope : forall x,
+  (* Equivalent to `(\x:0. 0) x`, in which the outer `x` is still free *)
+  fv_fast [] (TmAppl (TmForA (Some x) TmVoid TmVoid) (TmVarS x)) = [x].
+Proof. intros. simpl. Abort.
 
 (*
 Theorem fv_fast_slow_eq : forall t,
-  fv t = fv_slow t.
+  fv_slow t = rev (snd (fv_fast [] [] t)).
 Proof.
-  unfold fv. intros. induction t; intros; simpl in *;
-  try rewrite IHt1; try rewrite IHt2; simpl in *; try reflexivity.
+  intros t. induction t; intros; simpl in *; try reflexivity.
+  - destruct arg.
+    + destruct (fv_slow t2).
+      * rewrite app_nil_r. rewrite IHt1. destruct (fv_fast [] [] t1).
 Qed.
 
 Definition fv := fv_fast [].
 *)
 
 Definition fv := fv_slow.
+Arguments fv/ t.
+
+(* Crucial distinction from an easier-to-implement algorithm! *)
+Example fv_permits_shadowing : forall x,
+  (* Equivalent to `\x. \x. x x`, where the `x`s are distinct and pushed/popped in order. *)
+  fv (TmForA (Some x) TmVoid (TmForA (Some x) TmVoid (TmAppl (TmVarS x) (TmVarS x)))) = [].
+Proof. intros. simpl. repeat rewrite eqb_refl. reflexivity. Qed.
+
+(* Crucial distinction from an easier-to-implement algorithm! *)
+Example fv_permits_interrupted_shadowing : forall x y, y <> x ->
+  (* Equivalent to `\x. \y. \x. x x`, where the `x`s are distinct and pushed/popped in order. *)
+  fv (TmForA (Some x) TmVoid (TmForA (Some y) TmVoid (TmForA (Some x) TmVoid (TmAppl (TmVarS x) (TmVarS x))))) = [].
+Proof. intros. apply eqb_neq in H. simpl. rewrite eqb_refl. rewrite H. rewrite eqb_refl. reflexivity. Qed.
 
 Example fv_respects_scope : forall x,
   (* Equivalent to `(\x:0. 0) x`, in which the outer `x` is still free *)
@@ -107,10 +125,10 @@ Proof. intros. simpl. reflexivity. Qed.
 Inductive FreeIn : term -> list string -> Prop :=
   | FreeVoid :
       FreeIn TmVoid []
-  | FreeStar : forall lvl,
-      FreeIn (TmStar lvl) []
-  | FreeAtom : forall id lvl,
-      FreeIn (TmAtom id lvl) []
+  | FreeStar :
+      FreeIn TmStar []
+  | FreeAtom : forall id,
+      FreeIn (TmAtom id) []
   | FreeVarS : forall x,
       FreeIn (TmVarS x) [x]
   | FreePackNone : forall id ty curry va vb v,
@@ -161,29 +179,21 @@ Proof.
   induction hd; intros; simpl in *; try rewrite IHhd; reflexivity.
 Qed.
 
-(* Fantastic that we can prove something this precise! *)
-Theorem typed_requires_fv : forall ctx t ty,
-  Typed ctx t ty -> FreeIn t (map fst ctx).
-Proof.
-  intros. induction H; intros; simpl in *; subst; econstructor;
-  try apply IHTyped1; try apply IHTyped2; rewrite <- map_distr; reflexivity.
-Qed.
-
 Theorem reflect_fv : forall t v,
   FreeIn t v <-> fv t = v.
 Proof.
   split; intros.
   - induction H; intros; simpl in *; subst; try rewrite IHFreeIn2; try rewrite eqb_refl; try reflexivity;
-    destruct (fv curry); try reflexivity; destruct (eqb arg s) eqn:E; try reflexivity;
+    destruct (fv_slow curry); try reflexivity; destruct (eqb arg s) eqn:E; try reflexivity;
     rewrite eqb_eq in E; subst; contradiction H2; reflexivity.
   - generalize dependent v. induction t; intros; simpl in *; subst; try solve [econstructor].
-    + destruct arg; try (econstructor; try apply IHt1; try apply IHt2; reflexivity). destruct (fv t2).
+    + destruct arg; try (econstructor; try apply IHt1; try apply IHt2; reflexivity). destruct (fv_slow t2).
       { eapply FreePackDiff; try apply IHt1; try apply IHt2; try reflexivity. intro C. discriminate C. }
       destruct (eqb s s0) eqn:E.
       * apply eqb_eq in E. subst. econstructor; try apply IHt1; try apply IHt2; reflexivity.
       * apply eqb_neq in E. eapply FreePackDiff; try apply IHt1; try apply IHt2; try reflexivity.
         intro C. simpl in C. invert C. contradiction E. reflexivity.
-    + destruct arg; try (econstructor; try apply IHt1; try apply IHt2; reflexivity). destruct (fv t2).
+    + destruct arg; try (econstructor; try apply IHt1; try apply IHt2; reflexivity). destruct (fv_slow t2).
       { eapply FreeForADiff; try apply IHt1; try apply IHt2; try reflexivity. intro C. discriminate C. }
       destruct (eqb s s0) eqn:E.
       * apply eqb_eq in E. subst. econstructor; try apply IHt1; try apply IHt2; reflexivity.
@@ -192,9 +202,8 @@ Proof.
     + econstructor; try apply IHt1; try apply IHt2; reflexivity.
 Qed.
 
-Theorem fv_not_typed : forall t,
-  fv t <> [] -> ~exists ty, Typed [] t ty.
-Proof.
-  intros t H [ty C]. apply typed_requires_fv in C. apply reflect_fv in C.
-  rewrite C in H. contradiction H. reflexivity.
-Qed.
+Fixpoint str_in li s :=
+  match li with
+  | [] => false
+  | hd :: tl => if eqb s hd then true else str_in tl s
+  end.
