theories/Subst.v
@@ -1,347 +1,94 @@
 From Coq Require Import
   Lists.List.
 Import ListNotations.
-From Adam Require Import
+From Lang Require Import
+  Closed
   Invert
   Terms.
 
-Variant resource T := Unused | Used (output : T).
-Arguments Unused {T}.
-Arguments Used {T} output.
-
-Definition rmap : forall {A B}, (A -> B) -> resource A -> resource B := fun _ _ f r =>
-  match r with
-  | Unused => Unused
-  | Used x => Used (f x)
+Fixpoint smap
+  (f : (term -> term) -> term -> term)
+  (x : list (string * (term -> term))) :
+  list (string * (term -> term)) :=
+  match x with
+  | [] => []
+  | (s, g) :: tl => (s, f g) :: smap f tl
   end.
 
-Fixpoint count_free_slow x t :=
+Theorem smap_distr : forall f a b,
+  smap f (a ++ b) = smap f a ++ smap f b.
+Proof.
+  intros f a. generalize dependent f. induction a; intros; simpl in *.
+  { reflexivity. } destruct a. rewrite IHa. reflexivity.
+Qed.
+
+Theorem map_fst_smap : forall f li,
+  map fst (smap f li) = map fst li.
+Proof. induction li. { reflexivity. } destruct a. simpl. rewrite IHli. reflexivity. Qed.
+
+(* Ludicrous that this is the easiest correct definition to write.
+ * Generates substitution functions for every free variable at once. *)
+Fixpoint grand_unified_subst t : list (string * (term -> term)) :=
   match t with
+  | TmVoid
+  | TmStar
+  | TmAtom _ =>
+      []
   | TmVarS s =>
-      if eqb x s then 1 else 0
-  | TmPack _ None a b
-  | TmForA None a b
+      [(s, fun x => x)]
+  | TmPack id None a b =>
+      smap (fun f x => TmPack id None (f x) b) (grand_unified_subst a) ++
+      smap (fun f x => TmPack id None a (f x)) (grand_unified_subst b)
+  | TmForA None a b =>
+      smap (fun f x => TmForA None (f x) b) (grand_unified_subst a) ++
+      smap (fun f x => TmForA None a (f x)) (grand_unified_subst b)
   | TmAppl a b =>
-      count_free_slow x a + count_free_slow x b
-  | TmPack _ (Some arg) a b
-  | TmForA (Some arg) a b =>
-      if eqb x arg then 0 else
-      count_free_slow x a + count_free_slow x b
-  | _ => 0
-  end.
-Fixpoint count_free_fast acc x t :=
-  match t with
-  | TmVarS s =>
-      if eqb x s then S acc else acc
-  | TmPack _ None a b
-  | TmForA None a b
-  | TmAppl a b =>
-      count_free_fast (count_free_fast acc x a) x b
-  | TmPack _ (Some arg) a b
-  | TmForA (Some arg) a b =>
-      if eqb x arg then acc else
-      count_free_fast (count_free_fast acc x a) x b
-  | _ => acc
-  end.
-Lemma count_free_fast_acc_sum : forall x acc t,
-  count_free_fast acc x t = acc + count_free_fast 0 x t.
-Proof.
-  intros. generalize dependent x. generalize dependent acc.
-  induction t; intros; simpl in *; try rewrite Nat.add_0_r; try reflexivity.
-  - destruct (eqb x id) eqn:E; try rewrite Nat.add_0_r; try rewrite Nat.add_1_r; reflexivity.
-  - destruct arg.
-    + destruct (eqb x s) eqn:E. { rewrite Nat.add_0_r. reflexivity. }
-      rewrite IHt1. rewrite IHt2. rewrite <- Nat.add_assoc. f_equal. symmetry. apply IHt2.
-    + rewrite IHt2. rewrite IHt1. rewrite <- Nat.add_assoc. f_equal. symmetry. apply IHt2.
-  - destruct arg.
-    + destruct (eqb x s) eqn:E. { rewrite Nat.add_0_r. reflexivity. }
-      rewrite IHt1. rewrite IHt2. rewrite <- Nat.add_assoc. f_equal. symmetry. apply IHt2.
-    + rewrite IHt2. rewrite IHt1. rewrite <- Nat.add_assoc. f_equal. symmetry. apply IHt2.
-  - rewrite IHt2. rewrite IHt1. rewrite <- Nat.add_assoc. f_equal. symmetry. apply IHt2.
-Qed.
-Theorem count_free_eq : forall x t,
-  count_free_slow x t = count_free_fast 0 x t.
-Proof.
-  intros. generalize dependent x. induction t; intros; try reflexivity; simpl in *;
-  try (destruct arg; [destruct (eqb x s); [reflexivity |] |]);
-  rewrite count_free_fast_acc_sum; rewrite IHt1; rewrite IHt2; reflexivity.
-Qed.
-
-Inductive CountFree x : term -> nat -> Prop :=
-  | CountFreeVoid :
-      CountFree x TmVoid 0
-  | CountFreeStar : forall lvl,
-      CountFree x (TmStar lvl) 0
-  | CountFreeVarE :
-      CountFree x (TmVarS x) 1
-  | CountFreeVarD : forall s,
-      x <> s ->
-      CountFree x (TmVarS s) 0
-  | CountFreeAtom : forall id lvl,
-      CountFree x (TmAtom id lvl) 0
-  | CountFreePackNone : forall id ty curry a b c,
-      CountFree x ty a ->
-      CountFree x curry b ->
-      a + b = c ->
-      CountFree x (TmPack id None ty curry) c
-  | CountFreePackSomeE : forall id ty curry,
-      CountFree x (TmPack id (Some x) ty curry) 0
-  | CountFreePackSomeD : forall id s ty curry a b c,
-      x <> s ->
-      CountFree x ty a ->
-      CountFree x curry b ->
-      a + b = c ->
-      CountFree x (TmPack id (Some s) ty curry) c
-  | CountFreeForANone : forall ty body a b c,
-      CountFree x ty a ->
-      CountFree x body b ->
-      a + b = c ->
-      CountFree x (TmForA None ty body) c
-  | CountFreeForASomeE : forall ty body,
-      CountFree x (TmForA (Some x) ty body) 0
-  | CountFreeForASomeD : forall s ty body a b c,
-      x <> s ->
-      CountFree x ty a ->
-      CountFree x body b ->
-      a + b = c ->
-      CountFree x (TmForA (Some s) ty body) c
-  | CountFreeAppl : forall f y a b c,
-      CountFree x f a ->
-      CountFree x y b ->
-      a + b = c ->
-      CountFree x (TmAppl f y) c
-  .
-Theorem reflect_count_free_slow : forall x t n,
-  count_free_slow x t = n <-> CountFree x t n.
-Proof.
-  split; intros.
-  - generalize dependent x. generalize dependent n. induction t; intros; simpl in *; subst; try solve [constructor];
-    try (destruct arg; [destruct (eqb x s) eqn:E; [rewrite eqb_eq in E; subst; constructor |] |]);
-    try econstructor; try eapply IHt1; try eapply IHt2; try reflexivity;
-    try destruct (eqb x id) eqn:E; try rewrite eqb_eq in E; subst; try constructor; apply eqb_neq; assumption.
-  - induction H; simpl in *; repeat rewrite eqb_refl; try (apply eqb_neq in H; rewrite H);
-    try rewrite IHCountFree1; try rewrite IHCountFree2; try assumption; try reflexivity.
-Qed.
-Theorem reflect_count_free_fast : forall x t n,
-  count_free_fast 0 x t = n <-> CountFree x t n.
-Proof. intros. rewrite <- count_free_eq. apply reflect_count_free_slow. Qed.
-Definition count_free := count_free_fast 0.
-Arguments count_free/ x t.
-Theorem reflect_count_free : forall x t n,
-  count_free x t = n <-> CountFree x t n.
-Proof. intros. apply reflect_count_free_fast. Qed.
-
-(* Resource-aware substitution: substitute exactly once. *)
-Fixpoint subst pre post t :=
-  match t with
-  | TmVoid | TmStar _ | TmAtom _ _ => Unused
-  | TmVarS id => if eqb pre id then Used post else Unused
-  | TmPack id None ty curry =>
-      match subst pre post ty with
-      | Unused => rmap (TmPack id None ty) (subst pre post curry)
-      | Used ty' => Used (TmPack id None ty' curry)
+      smap (fun f x => TmAppl (f x) b) (grand_unified_subst a) ++
+      smap (fun f x => TmAppl a (f x)) (grand_unified_subst b)
+  | TmPack id (Some arg) ty curry =>
+      smap (fun f x => TmPack id (Some arg) (f x) curry) (grand_unified_subst ty) ++
+      smap (fun f x => TmPack id (Some arg) ty (f x))
+      match grand_unified_subst curry with
+      | [] => []
+      | (s, hd) :: tl => if eqb arg s then tl else (s, hd) :: tl
       end
-  | TmPack id (Some arg) ty curry => if eqb pre arg then Unused else
-      match subst pre post ty with
-      | Unused => rmap (TmPack id (Some arg) ty) (subst pre post curry)
-      | Used ty' => Used (TmPack id (Some arg) ty' curry)
-      end
-  | TmForA None ty body =>
-      match subst pre post ty with
-      | Unused => rmap (TmForA None ty) (subst pre post body)
-      | Used ty' => Used (TmForA None ty' body)
-      end
-  | TmForA (Some arg) ty body => if eqb pre arg then Unused else
-      match subst pre post ty with
-      | Unused => rmap (TmForA (Some arg) ty) (subst pre post body)
-      | Used ty' => Used (TmForA (Some arg) ty' body)
-      end
-  | TmAppl f x =>
-      match subst pre post f with
-      | Unused => rmap (TmAppl f) (subst pre post x)
-      | Used f' => Used (TmAppl f' x)
+  | TmForA (Some arg) ty curry =>
+      smap (fun f x => TmForA (Some arg) (f x) curry) (grand_unified_subst ty) ++
+      smap (fun f x => TmForA (Some arg) ty (f x))
+      match grand_unified_subst curry with
+      | [] => []
+      | (s, hd) :: tl => if eqb arg s then tl else (s, hd) :: tl
       end
   end.
-Inductive Subst (pre : string) (post : term) : term -> term -> Prop :=
-  | SubstVarE :
-      Subst pre post (TmVarS pre) post
-  | SubstPackNoneL : forall id ty ty' curry,
-      Subst pre post ty ty' ->
-      Subst pre post (TmPack id None ty curry) (TmPack id None ty' curry)
-  | SubstPackNoneR : forall id ty curry curry',
-      CountFree pre ty 0 ->
-      Subst pre post curry curry' ->
-      Subst pre post (TmPack id None ty curry) (TmPack id None ty curry')
-  | SubstPackSomeL : forall id arg ty ty' curry,
-      pre <> arg ->
-      Subst pre post ty ty' ->
-      Subst pre post (TmPack id (Some arg) ty curry) (TmPack id (Some arg) ty' curry)
-  | SubstPackSomeR : forall id arg ty curry curry',
-      pre <> arg ->
-      CountFree pre ty 0 ->
-      Subst pre post curry curry' ->
-      Subst pre post (TmPack id (Some arg) ty curry) (TmPack id (Some arg) ty curry')
-  | SubstForANoneL : forall ty ty' body,
-      Subst pre post ty ty' ->
-      Subst pre post (TmForA None ty body) (TmForA None ty' body)
-  | SubstForANoneR : forall ty body body',
-      CountFree pre ty 0 ->
-      Subst pre post body body' ->
-      Subst pre post (TmForA None ty body) (TmForA None ty body')
-  | SubstForASomeL : forall arg ty ty' body,
-      pre <> arg ->
-      Subst pre post ty ty' ->
-      Subst pre post (TmForA (Some arg) ty body) (TmForA (Some arg) ty' body)
-  | SubstForASomeR : forall arg ty body body',
-      pre <> arg ->
-      CountFree pre ty 0 ->
-      Subst pre post body body' ->
-      Subst pre post (TmForA (Some arg) ty body) (TmForA (Some arg) ty body')
-  | SubstApplL : forall f f' x,
-      Subst pre post f f' ->
-      Subst pre post (TmAppl f x) (TmAppl f' x)
-  | SubstApplR : forall f x x',
-      CountFree pre f 0 ->
-      Subst pre post x x' ->
-      Subst pre post (TmAppl f x) (TmAppl f x')
-  .
-(*
-Lemma subst_available_iff_never_used : forall pre post t,
-  Subst pre post t Unused <-> forall t', ~Subst pre post t (Used t').
+
+Fixpoint pair_lookup {V} key (pairs : list (string * V)) :=
+  match pairs with
+  | [] => None
+  | (k, v) :: tl => if eqb key k then Some v else pair_lookup key tl
+  end.
+
+Definition subst x y t := option_map (fun f => f y) (pair_lookup x (grand_unified_subst t)).
+Arguments subst x y t/.
+
+Example subst_simple : forall f x,
+  subst f TmStar (TmAppl (TmVarS f) x) = Some (TmAppl TmStar x).
+Proof. intros. simpl. rewrite eqb_refl. reflexivity. Qed.
+
+Example grand_unified_subst_simple :
+  grand_unified_subst (TmAppl (TmVarS "f"%string) (TmVarS "x"%string)) = [
+    ("f"%string, fun t => TmAppl t (TmVarS "x"%string));
+    ("x"%string, fun t => TmAppl (TmVarS "f"%string) t)].
+Proof. reflexivity. Qed.
+
+Theorem grand_unified_subst_exactly_fv : forall t,
+  fv t = map fst (grand_unified_subst t).
 Proof.
-  split; intros.
-  - intro C. generalize dependent t'. remember Unused as r eqn:E.
-    induction H; intros; simpl in *; invert E; invert C; try contradiction;
-    try solve [apply (IHSubst1 eq_refl ty'); assumption];
-    try solve [apply (IHSubst2 eq_refl curry'); assumption];
-    try solve [apply (IHSubst2 eq_refl body'); assumption];
-    try solve [apply (IHSubst1 eq_refl f'); assumption];
-    try solve [apply (IHSubst2 eq_refl x'); assumption].
-  - generalize dependent pre. generalize dependent post.
-    induction t; intros; simpl in *; try constructor.
-    + intros C. subst. contradiction (H post). constructor.
-    + destruct arg.
-      * destruct (eqb pre s) eqn:E. { rewrite eqb_eq in E. subst. constructor. }
-        rewrite eqb_neq in E. constructor; [assumption | apply IHt1 | apply IHt2];
-        intros t' C; eapply H. { apply SubstPackSomeL; [assumption | apply C]. }
-        apply SubstPackSomeR; [assumption | | apply C].
-        apply IHt1. intros t'' C'. eapply H. apply SubstPackSomeL. { assumption. } apply C'.
-      * constructor; [apply IHt1 | apply IHt2]; intros t' C; eapply H. { apply SubstPackNoneL. apply C. }
-        apply SubstPackNoneR; [| apply C]. apply IHt1. intros t'' C'. eapply H. apply SubstPackNoneL. apply C'.
-    + destruct arg.
-      * destruct (eqb pre s) eqn:E. { rewrite eqb_eq in E. subst. constructor. }
-        rewrite eqb_neq in E. constructor; [assumption | apply IHt1 | apply IHt2];
-        intros t' C; eapply H. { apply SubstForASomeL; [assumption | apply C]. }
-        apply SubstForASomeR; [assumption | | apply C].
-        apply IHt1. intros t'' C'. eapply H. apply SubstForASomeL. { assumption. } apply C'.
-      * constructor; [apply IHt1 | apply IHt2]; intros t' C; eapply H. { apply SubstForANoneL. apply C. }
-        apply SubstForANoneR; [| apply C]. apply IHt1. intros t'' C'. eapply H. apply SubstForANoneL. apply C'.
-    + apply IHt1. intros t' C. eapply H. constructor. apply C.
-    + apply IHt2. intros t' C. eapply H. apply SubstApplR; [| apply C].
-      apply IHt1. intros t'' C'. eapply H. constructor. apply C'.
+  intros t. induction t; intros; simpl in *; try reflexivity;
+  repeat rewrite IHt1; repeat rewrite IHt2; try destruct arg;
+  repeat rewrite map_distr; repeat rewrite map_fst_smap; f_equal;
+  destruct (grand_unified_subst t2); simpl in *; try reflexivity;
+  destruct p; simpl in *; destruct (eqb s s0); reflexivity.
 Qed.
-*)
+(* WOOHOOOOOOOOOOOOOOO *)
 
-Theorem subst_iff_count_nonzero_prop : forall pre post t,
-  count_free pre t = 0 <-> forall t', ~Subst pre post t t'.
-Proof.
-  split; intros.
-  - intro C. induction C; simpl in *; [rewrite eqb_refl in H; discriminate H | | | | | | | | | |];
-    rewrite count_free_fast_acc_sum in *;
-    try destruct (count_free_fast 0 pre f);
-    try destruct (count_free_fast 0 pre x);
-    try destruct (count_free_fast 0 pre ty);
-    try destruct (count_free_fast 0 pre body);
-    try destruct (count_free_fast 0 pre curry);
-    try (apply eqb_neq in H0; rewrite H0 in * );
-    try discriminate H; try apply (IHC eq_refl).
-  - generalize dependent pre. generalize dependent post. induction t; intros; simpl in *; try reflexivity;
-    try rewrite count_free_fast_acc_sum; try destruct arg;
-    try destruct (eqb pre s) eqn:Es; try apply eqb_neq in Es;
-    try erewrite IHt1; try erewrite IHt2; try reflexivity; try intros t' C; try eapply H;
-    try solve [constructor; try assumption; apply C];
-    try (apply SubstPackSomeR; [assumption | | apply C]);
-    try (apply SubstPackNoneR; [| apply C]);
-    try (apply SubstForASomeR; [assumption | | apply C]);
-    try (apply SubstForANoneR; [| apply C]);
-    try (apply SubstApplR; [| apply C]);
-    try apply reflect_count_free; try eapply IHt1; try eapply IHt2; try intros t'' C'; try eapply H;
-    try (constructor; try assumption; apply C').
-    destruct (eqb pre id) eqn:E; [| reflexivity]. apply eqb_eq in E. subst. contradiction (H post). constructor.
-Qed.
-
-Theorem reflect_not_subst : forall pre post t,
-  subst pre post t = Unused <-> forall t', ~Subst pre post t t'.
-Proof.
-  split; intros.
-  - intro C. generalize dependent H. induction C; intros; simpl in *;
-    try rewrite eqb_refl in *; try apply eqb_neq in H; try rewrite H in *;
-    try destruct (subst pre post ty); try destruct (subst pre post curry);
-    try destruct (subst pre post body); try destruct (subst pre post f); try destruct (subst pre post x);
-    try apply (IHC eq_refl); try discriminate.
-  - generalize dependent pre. generalize dependent post. induction t; intros; simpl in *; try reflexivity;
-    [destruct (eqb pre id) eqn:Ei; [| reflexivity]; apply eqb_eq in Ei; subst;
-      contradiction (H post); constructor | | |];
-    try (destruct arg; [destruct (eqb pre s) eqn:Es; [reflexivity |]; apply eqb_neq in Es |]);
-    (destruct (subst pre post t1) eqn:E1; [|
-      rewrite IHt1 in E1; [discriminate E1 |]; intros t' C; eapply H; constructor; try assumption; apply C]);
-    destruct (subst pre post t2) eqn:E2; try reflexivity; simpl in *;
-    (rewrite IHt2 in E2; [discriminate E2 |]); intros t' C; eapply H;
-    try apply SubstPackSomeR; try apply SubstPackNoneR;
-    try apply SubstForASomeR; try apply SubstForANoneR;
-    try apply SubstApplR; try assumption; try apply C;
-    apply reflect_count_free; apply subst_iff_count_nonzero_prop in H;
-    simpl in *; try (apply eqb_neq in Es; rewrite Es in H);
-    rewrite count_free_fast_acc_sum in H; (destruct (count_free_fast 0 pre t1); [reflexivity | discriminate H]).
-Qed.
-
-Theorem subst_iff_count_nonzero : forall pre post t,
-  count_free pre t = 0 <-> subst pre post t = Unused.
-Proof. intros. rewrite reflect_not_subst. apply subst_iff_count_nonzero_prop. Qed.
-
-Theorem reflect_subst : forall pre post t t',
-  subst pre post t = Used t' <-> Subst pre post t t'.
-Proof.
-  split; intros.
-  - generalize dependent pre. generalize dependent post. generalize dependent t'.
-    induction t; intros; simpl in *; subst; invert H;
-    [destruct (eqb pre id) eqn:E; [| discriminate]; rewrite eqb_eq in E; invert H1; constructor | | |];
-    try (destruct arg; [destruct (eqb pre s) eqn:E; [discriminate H1 |]; rewrite eqb_neq in E |]);
-    destruct (subst pre post t1) eqn:E1; try apply IHt1 in E1;
-    destruct (subst pre post t2) eqn:E2; try apply IHt2 in E2;
-    simpl in *; invert H1; constructor; try assumption;
-    apply reflect_count_free; eapply subst_iff_count_nonzero; apply E1.
-  - induction H; simpl in *; try rewrite eqb_refl; try rewrite <- eqb_neq in *; try rewrite IHSubst;
-    try rewrite <- reflect_count_free in *; try erewrite subst_iff_count_nonzero in *;
-    try rewrite H; try rewrite H0; reflexivity.
-Qed.
-
-(* TODO: Prove semantics are invariant to variable name changes! I'm not entirely sure `subst` is right. *)
-
-(* Crucial theorem! *)
-Theorem subst_exactly_once : forall pre post t t',
-  count_free pre post = 0 ->
-  subst pre post t = Used t' ->
-  count_free pre t = S (count_free pre t').
-Proof.
-  intros pre post t t' Hc Hs. repeat rewrite <- count_free_eq in *. apply reflect_subst in Hs.
-  induction Hs; simpl in *; try rewrite Hc; try rewrite IHHs;
-  try rewrite eqb_refl in *; try rewrite Nat.add_succ_r in *;
-  try rewrite <- eqb_neq in *; try rewrite H; reflexivity.
-Qed.
-
-(*
-Ideally, we would have a model of `forall` that
-naturally encoded the kind of linearity we want
-under Church encodings like in the C.o.C.:
-  - Arrow types are just anonymous `forall`s, so
-    an easy unit test is that we shouldn't be able to
-    reuse or ignore the argument of a `forall`.
-    Use it exactly once, and that's it.
-  - Next, (A, B) is represented ingeniously as
-    `forall C: Prop, (A -> B -> C) -> C`, i.e.
-    `forall C: Prop, forall _: (forall (_: A) (_: B), C), C`.
-    I think this would naturally allow us to
-    use each item exactly once as intended, but
-    it deserves more thought and a formal proof.
-*)
+(* TODO: Inductive equivalent *)
