theories/Typecheck.v
@@ -1,3 +1,14 @@
-From Adam Require Export
-  TypecheckDef
-  TypecheckFacts.
+From Lang Require Import
+  Terms.
+
+Variant TypecheckResult :=
+  | TCRVariable : string -> TypecheckResult
+  | TCRClosed : term -> TypecheckResult
+  .
+
+Print term.
+Fixpoint typecheck t :=
+  match t with
+  | TmVoid => TmStar
+  | TmStar => 
+  end.
